@prefix : <https://blue-room-innovation.github.io/bri-ontology/ontology/v0.1/digitalMarpolWastePassport.ttl#> .
@prefix owl: <http://www.w3.org/2002/07/owl#> .
@prefix rdf: <http://www.w3.org/1999/02/22-rdf-syntax-ns#> .
@prefix xml: <http://www.w3.org/XML/1998/namespace> .
@prefix xsd: <http://www.w3.org/2001/XMLSchema#> .
@prefix rdfs: <http://www.w3.org/2000/01/rdf-schema#> .

@base <https://blue-room-innovation.github.io/bri-ontology/ontology/v0.1/digitalMarpolWastePassport.ttl> .

<https://blue-room-innovation.github.io/bri-ontology/ontology/v0.1/digitalMarpolWastePassport.ttl> rdf:type owl:Ontology ;
                                                                   owl:imports <https://blue-room-innovation.github.io/bri-ontology/codelists/v0.1/delivery-type-code.ttl> ,
                                                                               <https://blue-room-innovation.github.io/bri-ontology/codelists/v0.1/discharge-means-code.ttl> ,
                                                                               <https://blue-room-innovation.github.io/bri-ontology/codelists/v0.1/iso3166-iAlpha2.ttl> ,
                                                                               <https://blue-room-innovation.github.io/bri-ontology/codelists/v0.1/residue-subtype-code.ttl> ,
                                                                               <https://blue-room-innovation.github.io/bri-ontology/codelists/v0.1/residue-type-code.ttl> ,
                                                                               <https://blue-room-innovation.github.io/bri-ontology/codelists/v0.1/unlocode.ttl> ;
                                                                   rdfs:comment "An ontology extending the Digital Waste Passport model for MARPOL-regulated waste documentation and reporting." ;
                                                                   rdfs:label "Digital MARPOL Waste Passport Ontology" ;
                                                                   owl:versionInfo "0.1" .

#################################################################
#    Annotation properties
#################################################################

###  http://www.w3.org/2004/02/skos/core#related
<http://www.w3.org/2004/02/skos/core#related> rdf:type owl:AnnotationProperty .


#################################################################
#    Object Properties
#################################################################

:contactPoint rdf:type owl:ObjectProperty ;
              rdfs:domain :AuthorizedParty ;
              rdfs:range <https://ontology.untp.io/core/Link> ;
              rdfs:comment "Contact information for the authorized party, represented as a link." .


:credentialSubject rdf:type owl:ObjectProperty ;
                   rdfs:domain :DigitalMarpolWastePassport ;
                   rdfs:range :MarpolWastePassport ;
                   rdfs:comment "References the MARPOL-specific waste passport subject (`MarpolWastePassport`)." .


:estimatedGenerated rdf:type owl:ObjectProperty ;
                    rdfs:domain :ResidueInformation ;
                    rdfs:range <https://ontology.untp.io/core/Measure> ;
                    rdfs:comment "The estimated quantity of residue generated, represented as a measure." .


:involvedParty rdf:type owl:ObjectProperty ;
               rdfs:domain :MarpolWaste ;
               rdfs:range :InvolvedParty ;
               rdfs:comment "The party involved in the waste management process, such as the ship operator or company." .


:maxCapacity rdf:type owl:ObjectProperty ;
             rdfs:domain :ResidueInformation ;
             rdfs:range <https://ontology.untp.io/core/Measure> ;
             rdfs:comment "The maximum capacity for residue storage, represented as a measure." .


:message rdf:type owl:ObjectProperty ;
         rdfs:domain :MarpolWaste ;
         rdfs:range :WasdisMetadata ;
         rdfs:comment "Metadata related to the WASDIS system, including the sender, message ID, and submission details." .


:quantityRemainingOnBoard rdf:type owl:ObjectProperty ;
                          rdfs:domain :ResidueInformation ;
                          rdfs:range <https://ontology.untp.io/core/Measure> ;
                          rdfs:comment "The quantity of residue still remaining onboard, represented as a measure." .


:quantityToDeliver rdf:type owl:ObjectProperty ;
                   rdfs:domain :ResidueInformation ;
                   rdfs:range <https://ontology.untp.io/core/Measure> ;
                   rdfs:comment "The quantity of residue to be delivered, represented as a measure." .


:residue rdf:type owl:ObjectProperty ;
         rdfs:domain :MarpolWaste ;
         rdfs:range :ResidueInformation ;
         rdfs:comment "Detailed information about the waste residue, including type, quantity, and discharge method." .


:role rdf:type owl:ObjectProperty ;
      rdfs:domain :InvolvedParty ;
      rdfs:range <https://ontology.untp.io/core/Party> ;
      rdfs:comment "The role of the involved party, as defined by the regulatory framework." .


:ship rdf:type owl:ObjectProperty ;
      rdfs:domain :MarpolWaste ;
      rdfs:range :Ship ;
      rdfs:comment "Details about the ship responsible for the waste, including the IMO number, name, and flag." .


:waste rdf:type owl:ObjectProperty ;
       rdfs:domain :MarpolWastePassport ;
       rdfs:range :MarpolWaste ;
       rdfs:comment "Details of the MARPOL-specific waste entity, encapsulating waste-related information within the MARPOL framework." .


:wasteAgent rdf:type owl:ObjectProperty ;
            rdfs:domain :MarpolWaste ;
            rdfs:range :AuthorizedParty ;
            rdfs:comment "The authorized waste collection company handling the waste." .


#################################################################
#    Data properties
#################################################################

:arrivalPort rdf:type owl:DatatypeProperty ;
             rdfs:domain :MarpolWaste ;
             rdfs:range xsd:string ;
             rdfs:comment "The port of arrival for the ship, identified using the UN/LOCODE format (e.g., `ESPMI`)." ;
             <http://www.w3.org/2004/02/skos/core#related> <https://blue-room-innovation.github.io/bri-ontology/codelists/v0.1/unlocode.ttl#UNLocodeScheme> .


:deliveryType rdf:type owl:DatatypeProperty ;
              rdfs:domain :MarpolWaste ;
              rdfs:range xsd:string ;
              rdfs:comment "Code indicating the type of delivery method used for the waste, based on a local codelist (e.g., `ZTO`)." ;
              <http://www.w3.org/2004/02/skos/core#related> <https://blue-room-innovation.github.io/bri-ontology/codelists/v0.1/delivery-type-code.ttl#DeliveryTypeCodeScheme> .


:dischargeMeans rdf:type owl:DatatypeProperty ;
                rdfs:domain :ResidueInformation ;
                rdfs:range xsd:string ;
                rdfs:comment "The method used to discharge the residue, identified by a local codelist code (e.g., `ZTE`)." ;
                <http://www.w3.org/2004/02/skos/core#related> <https://blue-room-innovation.github.io/bri-ontology/codelists/v0.1/discharge-means-code.ttl.ttl#DischargeMeansCodeScheme> .


:flag rdf:type owl:DatatypeProperty ;
      rdfs:domain :Ship ;
      rdfs:range xsd:string ;
      rdfs:comment "The flag state of the ship, identified by the ISO 3166-1 Alpha-2 code (e.g., `CY` for Cyprus)." ;
    <http://www.w3.org/2004/02/skos/core#related> <https://blue-room-innovation.github.io/bri-ontology/codelists/v0.1/iso3166-iAlpha2.ttl#ISO3166Alpha2Scheme> .



:identifier rdf:type owl:DatatypeProperty ;
            rdfs:domain :AuthorizedParty ;
            rdfs:range xsd:string ;
            rdfs:comment "A unique identifier for the authorized party." .


:imoNumber rdf:type owl:DatatypeProperty ;
           rdfs:domain :Ship ;
           rdfs:range xsd:string ;
           rdfs:comment "The International Maritime Organization (IMO) number, a 7-digit identifier for ships." .


:lastDeliveryDate rdf:type owl:DatatypeProperty ;
                  rdfs:domain :MarpolWaste ;
                  rdfs:range xsd:dateTime ;
                  rdfs:comment "The date and time of the last waste delivery, in ISO-8601 format with timezone." .


:lastWasteDeliveryPort rdf:type owl:DatatypeProperty ;
                       rdfs:domain :MarpolWaste ;
                       rdfs:range xsd:string ;
                       rdfs:comment "The last port where waste was delivered, using UN/LOCODE format." ;
                       <http://www.w3.org/2004/02/skos/core#related> <https://blue-room-innovation.github.io/bri-ontology/codelists/v0.1/unlocode.ttl#UNLocodeScheme> .


:marpolEdition rdf:type owl:DatatypeProperty ;
               rdfs:domain :MarpolWaste ;
               rdfs:range xsd:string ;
               rdfs:comment "The edition of MARPOL applicable to the waste being documented (if relevant)." .


:messageId rdf:type owl:DatatypeProperty ;
           rdfs:domain :WasdisMetadata ;
           rdfs:range xsd:string ;
           rdfs:comment "A unique identifier for the message." .


:name rdf:type owl:DatatypeProperty ;
      rdfs:domain :Ship ;
      rdfs:range xsd:string ;
      rdfs:comment "The name of the ship." .


:nextCollectionPort rdf:type owl:DatatypeProperty ;
                    rdfs:domain :ResidueInformation ;
                    rdfs:range xsd:string ;
                    rdfs:comment "The next port where the residue will be collected, identified by the UN/LOCODE" ;
                         <http://www.w3.org/2004/02/skos/core#related> <https://blue-room-innovation.github.io/bri-ontology/codelists/v0.1/unlocode.ttl#UNLocodeScheme> .


:nextPlannedDeliveryPort rdf:type owl:DatatypeProperty ;
                         rdfs:domain :MarpolWaste ;
                         rdfs:range xsd:string ;
                         rdfs:comment "The next planned port for waste delivery, identified with UN/LOCODE." ;
                         <http://www.w3.org/2004/02/skos/core#related> <https://blue-room-innovation.github.io/bri-ontology/codelists/v0.1/unlocode.ttl#UNLocodeScheme> .


:remarks rdf:type owl:DatatypeProperty ;
         rdfs:domain :WasdisMetadata ;
         rdfs:range xsd:string ;
         rdfs:comment "Any additional remarks or notes regarding the waste delivery or process." .


:sender rdf:type owl:DatatypeProperty ;
        rdfs:domain :WasdisMetadata ;
        rdfs:range xsd:string ;
        rdfs:comment "The entity that sent the waste notification." .


:shipScale rdf:type owl:DatatypeProperty ;
           rdfs:domain :MarpolWaste ;
           rdfs:range xsd:string ;
           rdfs:comment "An identifier for the ship scale or port call, useful for traceability." .


:submissionDate rdf:type owl:DatatypeProperty ;
                rdfs:domain :WasdisMetadata ;
                rdfs:range xsd:dateTime ;
                rdfs:comment "The date and time when the waste notification was submitted." .


:substance rdf:type owl:DatatypeProperty ;
           rdfs:domain :ResidueInformation ;
           rdfs:range xsd:string ;
           rdfs:comment "The substance of the residue, e.g., oil, sewage, or waste sludge." .


:subtypeCode rdf:type owl:DatatypeProperty ;
             rdfs:domain :ResidueInformation ;
             rdfs:range xsd:string ;
             rdfs:comment "Code representing the subtype of residue, providing more detailed categorization." ;
             <http://www.w3.org/2004/02/skos/core#related> <https://blue-room-innovation.github.io/bri-ontology/codelists/v0.1/residue-subtype-code.ttl#ResidueSubtypeCodeScheme> .


:typeCode rdf:type owl:DatatypeProperty ;
          rdfs:domain :ResidueInformation ;
          rdfs:range xsd:string ;
          rdfs:comment "Code representing the type of residue, based on a local codelist or MARPOL standard." ;
          <http://www.w3.org/2004/02/skos/core#related> <https://blue-room-innovation.github.io/bri-ontology/codelists/v0.1/residue-type-code.ttl#ResidueTypeCodeScheme> .


#################################################################
#    Classes
#################################################################

:AuthorizedParty rdf:type owl:Class ;
                 rdfs:comment "Represents an authorized entity responsible for handling the waste." .


:DigitalMarpolWastePassport rdf:type owl:Class ;
                            rdfs:subClassOf :DigitalWastePassport ;
                            rdfs:comment "A digital waste passport specific to MARPOL regulations, extending the generic `DigitalWastePassport`." .


:DigitalWastePassport rdf:type owl:Class .


:InvolvedParty rdf:type owl:Class ;
               rdfs:comment "A party involved in the waste management process, such as the ship operator." .


:MarpolWaste rdf:type owl:Class ;
             rdfs:subClassOf :Waste ;
             rdfs:comment "Represents a specific waste entity within the MARPOL context, including regulatory attributes for ship-generated waste." .


:MarpolWastePassport rdf:type owl:Class ;
                     rdfs:subClassOf :WastePassport ;
                     rdfs:comment "Represents the waste passport data specific to MARPOL regulations." .


:ResidueInformation rdf:type owl:Class ;
                    rdfs:comment "Details of a specific waste residue, including type, quantity, and handling." .


:Ship rdf:type owl:Class ;
      rdfs:comment "Details about the ship generating the waste." .


:WasdisMetadata rdf:type owl:Class ;
                rdfs:comment "Metadata related to the WASDIS system for auditing purposes." .


:Waste rdf:type owl:Class .


:WastePassport rdf:type owl:Class .


###  https://ontology.untp.io/core/Link
<https://ontology.untp.io/core/Link> rdf:type owl:Class .


###  https://ontology.untp.io/core/Measure
<https://ontology.untp.io/core/Measure> rdf:type owl:Class .


###  https://ontology.untp.io/core/Party
<https://ontology.untp.io/core/Party> rdf:type owl:Class .


###  Generated by the OWL API (version 4.5.29.2024-05-13T12:11:03Z) https://github.com/owlcs/owlapi
